![Hexagon Diagram](assets/hexagon_diag1.png)

In the diagram, \( `w` \) is the width of the hexagon, and \( `s` \) is the side length.

### Side Length `s`

In a regular hexagon, each side forms part of equilateral triangles, like triangle \( `ABC` \). The measure of angle \( `DBC` \) is 60 degrees, and the tangent of this angle is given by:

![Equation tan(60°) = |CD| / |DB|](https://latex.codecogs.com/svg.image?\inline&space;\LARGE&space;\bg{white}{\text{tan}(60^\circ)&space;=&space;\frac{|CD|}{|DB|}})

Since \( \text{tan}(60^\circ) = \sqrt{3} \), we can write:

![Equation tan(60°) = √3 = (w / 2) / (s / 2) = w / s](https://latex.codecogs.com/svg.image?\inline&space;\LARGE&space;\bg{white}{\text{tan}(60^\circ)&space;=&space;\sqrt{3}&space;=&space;\frac{w/2}{s/2}&space;=&space;\frac{w}{s}})

Thus, the relationship between the width \( `w` \) and the side length \( `s` \) is:

![Equation w = s√3](https://latex.codecogs.com/svg.image?\inline&space;\LARGE&space;\bg{white}{w&space;=&space;s\sqrt{3}})

### Solving for Side Length `s`

The side length \( `s` \) can be derived from the width \( `w` \) as:

![Equation s = w / √3](https://latex.codecogs.com/svg.image?\inline&space;\LARGE&space;\bg{white}{s&space;=&space;\frac{w}{\sqrt{3}}})

### Example Calculation

If the width \( `w` \) is given, you can calculate the side length using the above formula. For instance, if \( `w = 8` \) feet, then:

![Equation s = 8 / √3 ≈ 4.6 feet](https://latex.codecogs.com/svg.image?\inline&space;\LARGE&space;\bg{white}{s&space;=&space;\frac{8}{\sqrt{3}}&space;\approx&space;4.6\text{&space;feet}})

This general relationship allows you to determine the side length of any regular hexagon based on its width.

## References

[1] [mathcentral.uregina.ca 'Hexagon Tangent Problem'](https://mathcentral.uregina.ca/QQ/database/QQ.09.19/h/rob1.html)
